Implement SimpleInterface

theories/Simple.v
@@ -6,9 +6,12 @@ From Coq Require Import
      Morphisms.
 
 From ITree Require Import
-     Basics.Category
-     Basics.Basics
      Eq.Shallow.
+
+From ITree Require
+     Eq.UpToTaus
+     Interp.MorphismsFacts
+     Interp.RecursionFacts.
 (* end hide *)
 
 (** ** Core definitions *)
@@ -92,14 +95,14 @@ Global Declare Instance Equivalence_eutt :
     Equivalence eutt.
 
 (** We can erase taus unter [eutt]. *)
-Parameter eutt_tau : forall (t : itree E R),
+Parameter tau_eutt : forall (t : itree E R),
     Tau t ≈ t.
 
 Parameter itree_eta : forall (t : itree E R),
     t ≈ go (observe t).
 
 Parameter eutt_ret : forall (r1 r2 : R),
-    r1 = r2 <-> Ret r1 ≈ Ret r2.
+    Ret r1 ≈ Ret r2 <-> r1 = r2.
 
 Parameter eutt_vis : forall {U : Type} (e : E U) (k1 k2 : U -> itree E R),
     (forall u, k1 u ≈ k2 u) <-> Vis e k1 ≈ Vis e k2.
@@ -133,9 +136,8 @@ Parameter bind_bind
     ITree.bind (ITree.bind s k) h
   ≈ ITree.bind s (fun r => ITree.bind (k r) h).
 
-Hint Rewrite @eutt_tau : itree.
+Hint Rewrite @tau_eutt : itree.
 Hint Rewrite @ret_bind : itree.
-Hint Rewrite @tau_bind : itree.
 Hint Rewrite @vis_bind : itree.
 Hint Rewrite @bind_ret : itree.
 Hint Rewrite @bind_bind : itree.
@@ -241,7 +243,7 @@ Ltac tau_steps :=
       rewrite itree_eta at 1; cbn;
       match goal with
       | [ |- go (observe _) ≈ _ ] => fail 1
-      | _ => try rewrite eutt_tau
+      | _ => try rewrite tau_eutt
       end).
 
 End SimpleInterface.
@@ -258,26 +260,33 @@ Context {E : Type -> Type} {R : Type}.
 
 (** The standard [itree] equivalence: "Equivalence Up To Taus",
     or _weak bisimulation_. *)
-Parameter eutt : itree E R -> itree E R -> Prop.
+Definition eutt : itree E R -> itree E R -> Prop :=
+  ITree.Eq.UpToTaus.eutt eq.
 
 Infix "≈" := eutt (at level 40).
 
 (** [eutt] is an equivalence relation. *)
-Global Declare Instance Equivalence_eutt :
-    Equivalence eutt.
+Global Existing Instance UpToTaus.Equivalence_eutt.
 
 (** We can erase taus unter [eutt]. *)
-Parameter eutt_tau : forall (t : itree E R),
+Lemma tau_eutt : forall (t : itree E R),
     Tau t ≈ t.
+Proof. exact ITree.Eq.UpToTaus.tau_eutt. Qed.
 
-Parameter itree_eta : forall (t : itree E R),
+Lemma itree_eta : forall (t : itree E R),
     t ≈ go (observe t).
+Proof.
+  intros; rewrite <- ITree.Eq.Eq.itree_eta.
+  reflexivity.
+Qed.
 
-Parameter eutt_ret : forall (r1 r2 : R),
-    r1 = r2 <-> Ret r1 ≈ Ret r2.
+Lemma eutt_ret : forall (r1 r2 : R),
+    Ret r1 ≈ Ret r2 <-> r1 = r2.
+Proof. apply ITree.Eq.UpToTaus.eutt_ret. Qed.
 
-Parameter eutt_vis : forall {U : Type} (e : E U) (k1 k2 : U -> itree E R),
+Lemma eutt_vis : forall {U : Type} (e : E U) (k1 k2 : U -> itree E R),
     (forall u, k1 u ≈ k2 u) <-> Vis e k1 ≈ Vis e k2.
+Proof. apply ITree.Eq.UpToTaus.eutt_vis. Qed.
 
 End EquivalenceUpToTaus.
 
@@ -285,30 +294,35 @@ Infix "≈" := eutt (at level 40).
 
 (** *** Rewriting lemmas *)
 
-Parameter unfold_bind
+Lemma unfold_bind
   : forall {E R S} (t : itree E R) (k : R -> itree E S),
     ITree.bind t k
   ≈ ITree._bind k (fun t => ITree.bind t k) (observe t).
+Proof. intros; rewrite <- ITree.Eq.Shallow.unfold_bind; reflexivity. Qed.
 
 (** The next two are immediate corollaries of [unfold_bind]. *)
-Parameter ret_bind : forall {E R S} (r : R) (k : R -> itree E S),
+Lemma ret_bind : forall {E R S} (r : R) (k : R -> itree E S),
     ITree.bind (Ret r) k ≈ k r.
+Proof. intros; rewrite ITree.Eq.Shallow.ret_bind; reflexivity. Qed.
 
-Parameter vis_bind
+Lemma vis_bind
   : forall {E R} U V (e: E V) (ek: V -> itree E U) (k: U -> itree E R),
     ITree.bind (Vis e ek) k
   ≈ Vis e (fun x => ITree.bind (ek x) k).
+Proof. intros; rewrite ITree.Eq.Shallow.vis_bind; reflexivity. Qed.
 
-Parameter bind_ret : forall {E R} (s : itree E R),
+Lemma bind_ret : forall {E R} (s : itree E R),
     ITree.bind s (fun x => Ret x) ≈ s.
+Proof. intros; rewrite ITree.Eq.Eq.bind_ret; reflexivity. Qed.
 
-Parameter bind_bind
+Lemma bind_bind
   : forall {E R S T}
            (s : itree E R) (k : R -> itree E S) (h : S -> itree E T),
     ITree.bind (ITree.bind s k) h
   ≈ ITree.bind s (fun r => ITree.bind (k r) h).
+Proof. intros; rewrite ITree.Eq.Eq.bind_bind; reflexivity. Qed.
 
-Hint Rewrite @eutt_tau : itree.
+Hint Rewrite @tau_eutt : itree.
 Hint Rewrite @ret_bind : itree.
 Hint Rewrite @tau_bind : itree.
 Hint Rewrite @vis_bind : itree.
@@ -325,28 +339,46 @@ Definition _interp {E F} (f : E ~> itree F) R (ot : itreeF E R _)
      | VisF e k => Tau (f _ e >>= (fun x => interp f _ (k x)))
      end.
 
-Parameter unfold_interp
+Lemma unfold_interp
   : forall {E F R} {f : E ~> itree F} (t : itree E R),
     interp f _ t ≈ (_interp f _ (observe t)).
+Proof.
+  intros; rewrite <- ITree.Interp.MorphismsFacts.unfold_interp.
+  reflexivity.
+Qed.
 
-(** The next three are immediate corollaries of [unfold_interp]. *)
-Parameter ret_interp
+(** The next two are immediate corollaries of [unfold_interp]. *)
+Lemma ret_interp
   : forall {E F R} {f : E ~> itree F} (x: R),
     interp f _ (Ret x) ≈ Ret x.
+Proof.
+  intros; rewrite unfold_interp; reflexivity.
+Qed.
 
-Parameter vis_interp
+Lemma vis_interp
   : forall {E F R} {f : E ~> itree F} U (e: E U) (k: U -> itree E R),
     interp f _ (Vis e k)
   ≈ Tau (ITree.bind (f _ e) (fun x => interp f _ (k x))).
+Proof.
+  intros; rewrite unfold_interp; reflexivity.
+Qed.
 
-Parameter interp_lift : forall {E F : Type -> Type} {R : Type}
+Lemma interp_lift : forall {E F : Type -> Type} {R : Type}
       (f : E ~> (itree F)) (e : E R),
     interp f _ (ITree.lift e) ≈ f _ e.
+Proof.
+  intros; rewrite ITree.Interp.MorphismsFacts.interp_lift, tau_eutt.
+  reflexivity.
+Qed.
 
-Parameter interp_bind : forall {E F R S}
+Lemma interp_bind : forall {E F R S}
       (f : E ~> itree F) (t : itree E R) (k : R -> itree E S),
     interp f _ (ITree.bind t k)
   ≈ ITree.bind (interp f _ t) (fun r => interp f _ (k r)).
+Proof.
+  intros; rewrite ITree.Interp.MorphismsFacts.interp_bind.
+  reflexivity.
+Qed.
 
 (** **** Simple recursion: [rec] *)
 
@@ -356,15 +388,21 @@ Definition recursive {E A B} (f : A -> itree (callE A B +' E) B)
   : (callE A B +' E) ~> itree E
   := case_ (calling' (rec f)) ITree.lift.
 
-Parameter rec_as_interp
+Lemma rec_as_interp
   : forall {E A B} (f : A -> itree (callE A B +' E) B) (a : A),
     rec f a
   ≈ interp (recursive f) _ (f a).
+Proof.
+  intros; apply ITree.Interp.RecursionFacts.rec_as_interp.
+Qed.
 
-Parameter interp_recursive_call
+Lemma interp_recursive_call
   : forall {E A B} (f : A -> itree (callE A B +' E) B) (x : A),
     interp (recursive f) _ (call x)
   ≈ rec f x.
+Proof.
+  intros; apply ITree.Interp.RecursionFacts.interp_recursive_call.
+Qed.
 
 (** [mrec ctx] is equivalent to [interp (mrecursive ctx)],
     where [mrecursive] is defined as follows. *)
@@ -372,47 +410,60 @@ Definition mrecursive {D E} (f : D ~> itree (D +' E))
   : (D +' E) ~> itree E :=
   case_ (mrec f) ITree.lift.
 
-Parameter mrec_as_interp
+Lemma mrec_as_interp
   : forall {D E T} (ctx : D ~> itree (D +' E)) (d : D T),
     mrec ctx _ d
   ≈ interp (mrecursive ctx) _ (ctx _ d).
+Proof.
+  intros; apply ITree.Interp.RecursionFacts.mrec_as_interp.
+Qed.
 
-Parameter interp_mrecursive
+Lemma interp_mrecursive
   : forall {D E T} (ctx : D ~> itree (D +' E)) (d : D T),
     interp (mrecursive ctx) _ (lift_inl1 _ d)
   ≈ mrec ctx _ d.
+Proof.
+  intros; apply ITree.Interp.RecursionFacts.interp_mrecursive.
+Qed.
 
 (** *** [Proper] lemmas *)
 
-Declare Instance eutt_go {E R} :
+Instance eutt_go {E R} :
   Proper (going eutt ==> eutt) (@go E R).
+Proof. apply ITree.Eq.UpToTaus.eutt_cong_go. Qed.
 
-Declare Instance eutt_observe {E R} :
+Instance eutt_observe {E R} :
   Proper (eutt ==> going eutt) (@observe E R).
+Proof. apply ITree.Eq.UpToTaus.eutt_cong_observe. Qed.
 
-Declare Instance eutt_TauF {E R} :
+Instance eutt_TauF {E R} :
   Proper (eutt ==> going eutt) (@TauF E R _).
+Proof. apply ITree.Eq.UpToTaus.eutt_cong_tauF. Qed.
 
-Declare Instance eutt_VisF {E R X} (e: E X) :
+Instance eutt_VisF {E R X} (e: E X) :
   Proper (pointwise_relation _ (@eutt E R) ==> going eutt) (VisF e).
+Proof. apply ITree.Eq.UpToTaus.eutt_cong_VisF. Qed.
 
-Declare Instance eutt_bind {E R S} :
+Instance eutt_bind {E R S} :
   Proper (pointwise_relation _ eutt ==> eutt ==> eutt)
          (@ITree.bind' E R S).
+Proof. apply ITree.Eq.UpToTaus.eutt_bind. Qed.
 
-Declare Instance eutt_map {E R S} :
+Instance eutt_map {E R S} :
   Proper (pointwise_relation _ eq ==> eutt ==> eutt)
          (@ITree.map E R S).
+Proof. apply ITree.Eq.UpToTaus.eutt_map. Qed.
 
-Declare Instance eutt_interp (E F : Type -> Type) f (R : Type) :
+Instance eutt_interp (E F : Type -> Type) f (R : Type) :
   Proper (eutt ==> eutt) (@interp E F f R).
+Proof. apply ITree.Interp.MorphismsFacts.eutt_interp. Qed.
 
 Ltac tau_steps :=
   repeat (
       rewrite itree_eta at 1; cbn;
       match goal with
       | [ |- go (observe _) ≈ _ ] => fail 1
-      | _ => try rewrite eutt_tau
+      | _ => try rewrite tau_eutt
       end).
 
 End Simple.
